progress on multisorted experiments

theories_multisorted/Experiments.v
@@ -1,6 +1,77 @@
 From Prototype Require Import MPrelude MSig.
 
 (*********************************************************************************)
+(** *** Level one. *)
+(*********************************************************************************)
+
+Section LevelOne.
+Context {sig : signature}.
+
+Lemma occurs_in {s1 s2 ty} {c : fin (nctor s2)} : 
+  occurs_ty s1 ty -> In ty (ctor_type c) -> occurs s1 s2.
+Proof.
+intros H1 H2. apply occurs_base. exists c. rewrite Exists_exists. eauto.
+Qed.
+
+(** Level one terms. *)
+
+Inductive term : fin nsort -> Type :=
+| T_var {s} : has_var s -> nat -> term s
+| T_ctor {s} (c : fin (nctor s)) : args (ctor_type c) -> term s
+
+with args : list arg_ty -> Type :=
+| AL_nil : args []
+| AL_cons {ty tys} : arg ty -> args tys -> args (ty :: tys)
+
+with arg : arg_ty -> Type :=
+| A_base b : base_type b -> arg (AT_base b)
+| A_term {s} : term s -> arg (AT_term s)
+| A_bind {s s'} : term s' -> arg (AT_bind s s'). 
+
+Derive Signature NoConfusion NoConfusionHom for term args arg.
+
+Definition ren (s : fin nsort) := nat -> nat.
+
+(** Vector of renamings which can be applied to a term of sort [s]. *)
+Definition ren_vec (s : fin nsort) :=
+  forall s', occurs s' s -> has_var s' -> ren s'.
+
+(** Select a subvector of a vector of renaming. *)
+Equations? ren_subvector {s1 s2} (p : occurs s1 s2) (rv : ren_vec s2) : ren_vec s1 := 
+ren_subvector p rv := fun s' pocc pvar => rv s' _ pvar.
+Proof. eapply occurs_trans ; eauto. Qed.
+
+(** Apply a vector of renamings to a term. *)
+Equations? rename {s} (rv : ren_vec s) (t : term s) : term s :=
+rename rv (T_var p i) := T_var p (rv s (occurs_refl s) p i) ;
+rename rv (T_ctor c al) := T_ctor c (rename_args c _ rv al)
+
+with rename_args {s} {tys : list arg_ty} (c : fin (nctor s)) (p : incl tys (ctor_type c)) 
+  (rv : ren_vec s) (al : args tys) : args tys :=
+rename_args c p rv AL_nil := AL_nil ;
+rename_args c p rv (AL_cons a al) := AL_cons (rename_arg c _ rv a) (rename_args c _ rv al)
+
+with rename_arg {s} {ty : arg_ty} (c : fin (nctor s)) (p : In ty (ctor_type c))
+  (rv : ren_vec s) (a : arg ty) : arg ty :=
+rename_arg c p rv (A_base b x) := A_base b x ;
+rename_arg c p rv (A_term t) := A_term (rename (ren_subvector _ rv) t) ;
+rename_arg c p rv (A_bind a) := A_bind a.
+
+Proof.
+- apply p. now left.
+- apply p. now right.
+- unshelve eapply (occurs_in _ p). constructor.
+Qed.
+
+Lemma has_var_aux s : has_varb s -> has_var s.
+Proof. now destruct (has_var_spec s). Qed.
+
+Lemma has_var_aux' s : has_var s -> has_varb s.
+Proof. now destruct (has_var_spec s). Qed.
+
+End LevelOne.
+
+(*********************************************************************************)
 (** *** Level zero. *)
 (*********************************************************************************)
 
@@ -19,63 +90,140 @@ with vl : Type :=
 | lam : ty -> tm -> vl
 | tlam : tm -> vl.
 
-Equations rename_ty (rty : ren) : ty -> ty :=
+Equations rename_ty (rty : nat -> nat) : ty -> ty :=
 rename_ty rty (var_ty i) := var_ty (rty i) ;
 rename_ty rty (arr t1 t2) := arr (rename_ty rty t1) (rename_ty rty t2) ;
 rename_ty rty (all t) := all (rename_ty (up_ren rty) t).
 
-Equations rename_tm (rty : ren) (rvl : ren) : tm -> tm :=
+Equations rename_tm (rty rvl : nat -> nat) : tm -> tm :=
 rename_tm rty rvl (app t1 t2) := app (rename_tm rty rvl t1) (rename_tm rty rvl t2) ;
 rename_tm rty rvl (tapp t1 t2) := tapp (rename_tm rty rvl t1) (rename_ty rty t2) ;
 rename_tm rty rvl (vt v) := vt (rename_vl rty rvl v)
 
-with rename_vl (rty : ren) (rvl : ren) : vl -> vl :=
+with rename_vl (rty rvl : nat -> nat) : vl -> vl :=
 rename_vl rty rvl (var_vl i) := var_vl (rvl i) ;
 rename_vl rty rvl (lam t1 t2) := lam (rename_ty rty t1) (rename_tm rty (up_ren rvl ) t2) ;
 rename_vl rty rvl (tlam t) := tlam (rename_tm (up_ren rty) rvl t).
 
-
-
 (*********************************************************************************)
-(** *** Level one. *)
+(** *** Signature. *)
 (*********************************************************************************)
 
-Section Sec.
-Context (sig : signature).
+Definition nbase_ := 0.
 
-(** [occurs_aux] *)
+Definition base_type_ (b : fin nbase_) : Type :=
+  vector_nth b vnil.
 
-Inductive occurs_aux (s : fin nsort) : @arg_ty nbase nsort -> Prop :=
-| occurs_aux_term : occurs_aux s (AT_term s)
-| occurs_aux_bind {s' ty} : occurs_aux s ty -> occurs_aux s (AT_bind s' ty).
+Definition nsort_ := 3.
+Notation sty := (finO) (only parsing).
+Notation stm := (finS finO) (only parsing).
+Notation svl := (finS (finS finO)) (only parsing).
 
-Equations occurs_auxb : fin nsort -> @arg_ty nbase nsort -> bool :=
-occurs_auxb s (AT_base _) := false ;
-occurs_auxb s (AT_term s') := eqb_fin s s' ;
-occurs_auxb s (AT_bind _ ty) := occurs_auxb s ty.
+Definition nctor_ (s : fin nsort_) : nat :=
+  vector_nth s (vcons 2 (vcons 3 (vcons 2 vnil))).
 
-Lemma occurs_aux_spec s ty : reflect (occurs_aux s ty) (occurs_auxb s ty).
-Proof. Admitted.
+Equations ctor_type_ (s : fin nsort_) (c : fin (nctor_ s)) : list (@arg_ty nbase_ nsort_) :=
+ctor_type_ sty c := 
+  vector_nth c [| [ AT_term sty ; AT_term sty ] ; [ AT_bind sty sty ] |] ;
+ctor_type_ _ _ := [].
 
-(** [occurs] *)
+ctor_type_ stm finO := [ AT_term stm ; AT_term stm ] ;
+ctor_type_ stm (finS finO) := [ AT_term stm ; AT_term sty ] ;
+ctor_type_ stm (finS (finS finO)) := [ AT_term svl ] ;
 
-Equations fin_existsb (n : nat) (P : fin n -> bool) : bool :=
-fin_existsb 0 _ := false ;
-fin_existsb (S n) P := P finO || fin_existsb n (fun i => P (finS i)).
+ctor_type_ svl finO := [ AT_term sty ; AT_bind svl stm ] ;
+ctor_type_ svl (finS finO) := [ AT_bind sty stm ].
 
-Definition occurs (s s' : fin nsort) : Prop :=
-  exists c : fin (nctor s'), Exists (occurs_aux s) (ctor_type c).
+Definition sig : signature := 
+  Build_signature nbase_ base_type_ nsort_ nctor_ ctor_type_.
 
-Definition occursb (s s' : fin nsort) : bool :=
-  fin_existsb (nctor s') (fun c => existsb (occurs_auxb s) (ctor_type c)).
-  
-Lemma occurs_spec s s' : reflect (occurs s s') (occursb s s').
-Proof. Admitted. 
+(*********************************************************************************)
+(** *** Bijection between level zero and one. *)
+(*********************************************************************************)
 
-(* TODO: transitive closure of [occurs]. *)
+Lemma explode {A : Type} : is_true false -> A.
+Proof. intros H. unfold is_true in H. discriminate. Qed.
 
-(** [binds_aux] *)
+Equations reify_ty : ty -> @term sig sty :=
+reify_ty (var_ty i) := T_var (@has_var_aux sig sty eq_refl) i ;
+reify_ty (arr t1 t2) := 
+  @T_ctor sig sty finO (AL_cons (A_term (reify_ty t1)) (AL_cons (A_term (reify_ty t2)) AL_nil)) ;
+reify_ty (all t) := 
+  @T_ctor sig sty (finS finO) (AL_cons (A_bind (reify_ty t)) AL_nil).
 
-Inductive binds_aux (s : fin nsort) : @arg_ty nbase nsort -> Prop :=
-| binds_aux_base {ty} : binds_aux s (AT_bind s ty)
-| binds_aux_step {s' ty} : binds_aux s ty -> binds_aux s (AT_bind s' ty).
+Equations reify_tm : tm -> @term sig stm :=
+reify_tm (app t1 t2) :=
+  @T_ctor sig stm finO (AL_cons (A_term (reify_tm t1)) (AL_cons (A_term (reify_tm t2)) AL_nil)) ;
+reify_tm (tapp t1 t2) :=
+  @T_ctor sig stm (finS finO) (AL_cons (A_term (reify_tm t1)) (AL_cons (A_term (reify_ty t2)) AL_nil)) ;
+reify_tm (vt t) :=
+  @T_ctor sig stm (finS (finS finO)) (AL_cons (A_term (reify_vl t)) AL_nil)
+
+with reify_vl : vl -> @term sig svl :=
+reify_vl (var_vl i) := T_var (@has_var_aux sig svl eq_refl) i ;
+reify_vl (lam t1 t2) :=
+  @T_ctor sig svl finO (AL_cons (A_term (reify_ty t1)) (AL_cons (A_bind (reify_tm t2)) AL_nil)) ;
+reify_vl (tlam t) :=
+  @T_ctor sig svl (finS finO) (AL_cons (A_bind (reify_tm t)) AL_nil).
+
+Equations eval_sort (s : fin (@nsort sig)) : Type :=
+eval_sort sty := ty ;
+eval_sort stm := tm ;
+eval_sort svl := vl.
+
+Equations eval_arg_ty (ty : @arg_ty (@nbase sig) (@nsort sig)) : Type :=
+eval_arg_ty (AT_base b) := @base_type sig b ;
+eval_arg_ty (AT_term s) := eval_sort s ;
+eval_arg_ty (AT_bind _ s) := eval_sort s.
+
+Equations eval_arg_tys (tys : list (@arg_ty (@nbase sig) (@nsort sig))) : Type :=
+eval_arg_tys [] := unit ;
+eval_arg_tys (ty :: tys) := eval_arg_ty ty * eval_arg_tys tys.
+
+Equations eval_ctor (s : fin (@nsort sig)) (c : fin (nctor s)) : 
+  eval_arg_tys (ctor_type c) -> eval_sort s :=
+eval_ctor sty finO (t1, (t2, tt)) := arr t1 t2 ;
+eval_ctor sty (finS finO) (t, tt) := all t ;
+
+eval_ctor stm finO (t1, (t2, tt)) := app t1 t2 ;
+eval_ctor stm (finS finO) (t1, (t2, tt)) := tapp t1 t2 ;
+eval_ctor stm (finS (finS finO)) (t, tt) := vt t ;
+
+eval_ctor svl finO (t1, (t2, tt)) := lam t1 t2 ;
+eval_ctor svl (finS finO) (t, tt) := tlam t.
+
+Equations eval {s} : @term sig s -> eval_sort s :=
+@eval sty (T_var p i) := var_ty i ;
+@eval stm (T_var p _) := explode (has_var_aux' _ p) ;
+@eval svl (T_var _ i) := var_vl i ;
+eval (T_ctor c al) := eval_ctor s c (eval_args al)
+
+with eval_args {tys} (al : args tys) : eval_arg_tys tys :=
+eval_args AL_nil := tt ;
+eval_args (AL_cons a al) := (eval_arg a, eval_args al)
+
+with eval_arg {ty} (a : arg ty) : eval_arg_ty ty :=
+eval_arg (A_base b x) := x ;
+eval_arg (A_term t) := eval t ;
+eval_arg (A_bind t) := eval t.
+
+Lemma eval_reify_ty (t : ty) : eval (reify_ty t) = t.
+Proof.
+induction t ; simp reify_ty eval.
+- reflexivity.
+- change (@ctor_type sig (@finO 2) (@finO 1)) with 
+    [@AT_term nbase_ nsort_ sty ; AT_term sty].
+  simp eval. rewrite IHt1, IHt2. reflexivity.
+- change (@ctor_type sig (@finO 2) (@finS 1 (@finO 0))) with 
+    [@AT_bind nbase_ nsort_ sty sty].
+  simp eval. rewrite IHt. reflexivity.
+Qed.
+
+Lemma eval_reify_tm : 
+  (forall t, eval (reify_tm t) = t) * (forall v, eval (reify_vl v) = v).
+Proof.
+apply reify_tm_elim with 
+  (P := fun t res => eval res = t)
+  (P0 := fun v res => eval res = v).
+- intros t1 t2 H1 H2. simp eval. Set Printing Implicit.
+Admitted.
